---
title: W3 Hyperbolic Functions
---

## Even/Odd Functions

- Even Function
  - $\boxed{f(-x)=f(x)}$
  - symmetrical over $y$-axis
- Odd Function
  - $\boxed{f(-x)=-f(x)}$
  - flipped over $y$ and $x$ axis

## Hyperbolic Functions

|                       graph                        |                            function                             | domain($x$) |  range($y$)  |
| :------------------------------------------------: | :-------------------------------------------------------------: | :---------: | :----------: |
| ![](/src/assets/mast10006/2021-03-27-11-22-21.png) |                 $\sinh x=\frac{e^x-e^{-x}}{2}$                  |    $\R$     |     $\R$     |
| ![](/src/assets/mast10006/2021-03-27-11-23-12.png) |                 $\cosh x=\frac{e^x+e^{-x}}{2}$                  |    $\R$     | $[1,\infty]$ |
| ![](/src/assets/mast10006/2021-03-27-11-24-01.png) | $\tanh x=\frac{\sinh x}{\cosh x}=\frac{e^x-e^{-x}}{e^x+e^{-x}}$ |    $\R$     |   $(-1,1)$   |

## Reciprocal Hyperbolic Functions

|                       graph                        |                         function                         |         domain($x$)          |           range($y$)           |
| :------------------------------------------------: | :------------------------------------------------------: | :--------------------------: | :----------------------------: |
| ![](/src/assets/mast10006/2021-03-27-11-32-24.png) | $\textmd{csch }x=\frac{1}{\sinh x}=\frac{2}{e^x-e^{-x}}$ |        $\R$ \ $\{0\}$        |         $\R$ \ $\{0\}$         |
| ![](/src/assets/mast10006/2021-03-27-11-34-01.png) | $\textmd{sech }x=\frac{1}{\cosh x}=\frac{2}{e^x+e^{-x}}$ |             $\R$             |          $( 0, 1] \,$          |
| ![](/src/assets/mast10006/2021-03-27-11-26-46.png) |            $\coth x=\frac{\cosh x}{\sinh x}$             | $(-\infty,0)\cup(0, \infty)$ | $(-\infty,-1)\cup(1), \infty)$ |
|                                                    |                                                          |                              |

## Inverse Hyperbolic Functions

> Derivation: [Derivation of Inverse Hyperbolic Functions](https://github.com/chuahxinyu/notezzz/blob/main/src/assets/mast10006/derive-inverse-hyperbolic.pdf)

- $\textmd{arcsinh }u=\log (u+\sqrt{u^2+1})\frac{du}{dx}$
- $\textmd{arccosh }u=\log (u+\sqrt{u^2-1})\frac{du}{dx}$
- $\textmd{arctanh }u=\frac{1}{3}\log(\frac{1+u}{1-u})\frac{du}{dx}$

- $\textmd{arccsch }u=-\frac{1}{|u|\sqrt{1+u^2}}\frac{du}{dx}$
- $\textmd{arcsech }u=-\frac{1}{u\sqrt{1-u^2}}\frac{du}{dx}$
- $\textmd{arccoth }u=\frac{1}{1-u^2}\frac{du}{dx}$

## Inverse Reciprocal Hyperbolic Functions

## Hyperbolic Formulae

- $\tanh x=\frac{\sinh x}{\cosh x}$

### Sum/Difference Formulae

- $\sinh(x+y)=\sinh x\cosh y+\cosh x\sinh y$
- $\cosh(x+y)=\cosh x\cosh y+\sinh x\sinh y$
- $\sinh(x-y)=\sinh x\cosh y-\cosh x\sinh y$
- $\cosh(x-y)=\cosh x\cosh y=\sinh x\sinh y$

### Double angle Formulae

- $\sinh(2x)=2\sinh(x)\cosh(x)$
- $\cosh(2x)=\cosh^2(x)+\sinh^2(x)$
- $\cosh(2x)=2\cosh^2(x)-1$
- $\cosh(2x)=2\sinh^2(x)+1$

### Basic Identities

- $\cosh^2(x)-\sinh^2(x)=1$
- $\coth^2(x)-1=\textmd{cosech}^2(x)$
- $1-\tanh^2(x)=\textmd{sech}^2(x)$

## Derivatives

- $\frac{d}{dx}(\sinh u)=\cosh u \times\frac{du}{dx}$
- $\frac{d}{dx}(\textmd{cosh }u)=\sinh u \times\frac{du}{dx}$
- $\frac{d}{dx}(\tanh u)=\textmd{sech}^2u \times\frac{du}{dx}$

---

- $\frac{d}{dx}(\textmd{csch }u)=-\textmd{csch }u\times\frac{du}{dx}$
- $\frac{d}{dx}(\textmd{sech }u)=-\textmd{sech }u\tanh u\frac{du}{dx}$
- $\frac{d}{dx}(\textmd{coth }u)=-\textmd{csch}^2u\frac{du}{dx}$

---

- $\frac{d}{dx}(\textmd{arcsinh }x)=\frac{1}{\sqrt{x^2+1}}$
- $\frac{d}{dx}(\textmd{arccosh }x)=\frac{1}{\sqrt{x^2-1}}$
- $\frac{d}{dx}(\textmd{arctanh }x)=\frac{1}{1-x^2}$
